src/lib/data/Kuiper.Matrix4.fst
@@ -468,7 +468,7 @@ fn gpu_matrix_explode
       A.varray_pts_to_cell gm #f rc ((aview_from_mlayout et l).igm.acc em rc))
     (fun rc ->
       A.varray_pts_to_cell gm #f (rc._1, rc._2) (EMatrix.macc em rc._1 rc._2));
-  forevery_unflatten #(natlt (mrows * brows)) #_ #(natlt (mcols * bcols))
+  forevery_unflatten #(natlt (mrows * brows)) #(natlt (mcols * bcols))
     (fun r c ->
       A.varray_pts_to_cell gm #f (r, c) (EMatrix.macc em r c));
   forevery_factor (mrows * brows) mrows brows _;
